Fin74.lean
@@ -4,6 +4,8 @@ public import Fin74.Formula.Basic
 public import Fin74.Formula.Substitution
 public import Fin74.Kripke.Basic
 public import Fin74.Kripke.Chain
-public import Fin74.Lemma1.Basic
 public import Fin74.Logic.Basic
-public import Fin74.Logic.Shift
+public import Fin74.Result.Incomplete
+public import Fin74.Result.Model
+public import Fin74.Result.ModelForcing
+public import Fin74.Result.ValidatesG
